libcrux-ml-kem/src/vector/portable/vector_type.rs
@@ -11,6 +11,7 @@ pub struct PortableVector {
 
 #[allow(non_snake_case)]
 #[inline(always)]
+#[hax_lib::ensures(|result| fstar!("to_i16_array $result == Seq.create 16 0s"))]
 pub fn zero() -> PortableVector {
     PortableVector {
         elements: [0i16; FIELD_ELEMENTS_IN_VECTOR],
@@ -18,13 +19,15 @@ pub fn zero() -> PortableVector {
 }
 
 #[inline(always)]
+#[hax_lib::ensures(|result| fstar!("${result} == ${x}.f_elements"))]
+pub fn to_i16_array(x: PortableVector) -> [i16; 16] {
+    x.elements
+}
+
+#[inline(always)]
+#[hax_lib::ensures(|result| fstar!("${result}.f_elements == $array"))]
 pub fn from_i16_array(array: &[i16]) -> PortableVector {
     PortableVector {
         elements: array[0..16].try_into().unwrap(),
     }
-}
-
-#[inline(always)]
-pub fn to_i16_array(x: PortableVector) -> [i16; 16] {
-    x.elements
 }
