libcrux-ml-kem/proofs/fstar/extraction/Libcrux_ml_kem.Vector.Avx2.fst
@@ -3,15 +3,33 @@ module Libcrux_ml_kem.Vector.Avx2
 open Core
 open FStar.Mul
 
+let _ =
+  (* This module has implicit dependencies, here we make them explicit. *)
+  (* The implicit dependencies arise from typeclasses instances. *)
+  let open Libcrux_ml_kem.Vector.Traits in
+  ()
+
+let repr (x:t_SIMD256Vector) = admit()
+
 let from_i16_array (array: t_Slice i16) =
-  { f_elements = Libcrux_intrinsics.Avx2_extract.mm256_loadu_si256_i16 array } <: t_SIMD256Vector
+  let result:t_SIMD256Vector =
+    { f_elements = Libcrux_intrinsics.Avx2_extract.mm256_loadu_si256_i16 array } <: t_SIMD256Vector
+  in
+  let _:Prims.unit = admit () (* Panic freedom *) in
+  result
 
 let to_i16_array (v: t_SIMD256Vector) =
   let output:t_Array i16 (sz 16) = Rust_primitives.Hax.repeat 0s (sz 16) in
   let output:t_Array i16 (sz 16) =
     Libcrux_intrinsics.Avx2_extract.mm256_storeu_si256_i16 output v.f_elements
   in
-  output
+  let result:t_Array i16 (sz 16) = output in
+  let _:Prims.unit = admit () (* Panic freedom *) in
+  result
 
 let zero (_: Prims.unit) =
-  { f_elements = Libcrux_intrinsics.Avx2_extract.mm256_setzero_si256 () } <: t_SIMD256Vector
+  let result:t_SIMD256Vector =
+    { f_elements = Libcrux_intrinsics.Avx2_extract.mm256_setzero_si256 () } <: t_SIMD256Vector
+  in
+  let _:Prims.unit = admit () (* Panic freedom *) in
+  result
