libcrux-ml-kem/proofs/fstar/extraction/Libcrux_ml_kem.Vector.Neon.Vector_type.fsti
@@ -8,10 +8,28 @@ type t_SIMD128Vector = {
   f_high:u8
 }
 
-val v_ZERO: Prims.unit -> Prims.Pure t_SIMD128Vector Prims.l_True (fun _ -> Prims.l_True)
+val repr (x:t_SIMD128Vector) : t_Array i16 (sz 16)
 
-val from_i16_array (array: t_Slice i16)
-    : Prims.Pure t_SIMD128Vector Prims.l_True (fun _ -> Prims.l_True)
+val v_ZERO: Prims.unit
+  -> Prims.Pure t_SIMD128Vector
+      Prims.l_True
+      (ensures
+        fun result ->
+          let result:t_SIMD128Vector = result in
+          repr result == Seq.create 16 0s)
 
 val to_i16_array (v: t_SIMD128Vector)
-    : Prims.Pure (t_Array i16 (sz 16)) Prims.l_True (fun _ -> Prims.l_True)
+    : Prims.Pure (t_Array i16 (sz 16))
+      Prims.l_True
+      (ensures
+        fun result ->
+          let result:t_Array i16 (sz 16) = result in
+          result == repr v)
+
+val from_i16_array (array: t_Slice i16)
+    : Prims.Pure t_SIMD128Vector
+      Prims.l_True
+      (ensures
+        fun result ->
+          let result:t_SIMD128Vector = result in
+          repr result == array)
