libcrux-ml-kem/proofs/fstar/extraction/Libcrux_ml_kem.Vector.Portable.fsti
@@ -7,27 +7,36 @@ let _ =
   (* This module has implicit dependencies, here we make them explicit. *)
   (* The implicit dependencies arise from typeclasses instances. *)
   let open Libcrux_ml_kem.Vector.Portable.Vector_type in
+  let open Libcrux_ml_kem.Vector.Traits in
   ()
 
 [@@ FStar.Tactics.Typeclasses.tcinstance]
-let impl: Libcrux_ml_kem.Vector.Traits.t_Operations
+let impl: Libcrux_ml_kem.Vector.Traits.t_Repr
 Libcrux_ml_kem.Vector.Portable.Vector_type.t_PortableVector =
   {
     _super_11581440318597584651 = FStar.Tactics.Typeclasses.solve;
     _super_9442900250278684536 = FStar.Tactics.Typeclasses.solve;
-    f_ZERO_pre = (fun (_: Prims.unit) -> true);
-    f_ZERO_post
+    f_repr_pre = (fun (x: Libcrux_ml_kem.Vector.Portable.Vector_type.t_PortableVector) -> true);
+    f_repr_post
     =
-    (fun (_: Prims.unit) (out: Libcrux_ml_kem.Vector.Portable.Vector_type.t_PortableVector) -> true);
-    f_ZERO = (fun (_: Prims.unit) -> Libcrux_ml_kem.Vector.Portable.Vector_type.zero ());
-    f_from_i16_array_pre = (fun (array: t_Slice i16) -> true);
-    f_from_i16_array_post
-    =
-    (fun (array: t_Slice i16) (out: Libcrux_ml_kem.Vector.Portable.Vector_type.t_PortableVector) ->
+    (fun
+        (x: Libcrux_ml_kem.Vector.Portable.Vector_type.t_PortableVector)
+        (out: t_Array i16 (sz 16))
+        ->
         true);
-    f_from_i16_array
+    f_repr
     =
-    (fun (array: t_Slice i16) -> Libcrux_ml_kem.Vector.Portable.Vector_type.from_i16_array array);
+    fun (x: Libcrux_ml_kem.Vector.Portable.Vector_type.t_PortableVector) ->
+      Libcrux_ml_kem.Vector.Portable.Vector_type.to_i16_array x
+  }
+
+[@@ FStar.Tactics.Typeclasses.tcinstance]
+let impl_1: Libcrux_ml_kem.Vector.Traits.t_Operations
+Libcrux_ml_kem.Vector.Portable.Vector_type.t_PortableVector =
+  {
+    _super_11581440318597584651 = FStar.Tactics.Typeclasses.solve;
+    _super_9442900250278684536 = FStar.Tactics.Typeclasses.solve;
+    _super_8706949974463268012 = FStar.Tactics.Typeclasses.solve;
     f_to_i16_array_pre
     =
     (fun (x: Libcrux_ml_kem.Vector.Portable.Vector_type.t_PortableVector) -> true);
@@ -37,11 +46,27 @@ Libcrux_ml_kem.Vector.Portable.Vector_type.t_PortableVector =
         (x: Libcrux_ml_kem.Vector.Portable.Vector_type.t_PortableVector)
         (out: t_Array i16 (sz 16))
         ->
-        true);
+        out == impl.f_repr x);
     f_to_i16_array
     =
     (fun (x: Libcrux_ml_kem.Vector.Portable.Vector_type.t_PortableVector) ->
         Libcrux_ml_kem.Vector.Portable.Vector_type.to_i16_array x);
+    f_ZERO_pre = (fun (_: Prims.unit) -> true);
+    f_ZERO_post
+    =
+    (fun (_: Prims.unit) (out: Libcrux_ml_kem.Vector.Portable.Vector_type.t_PortableVector) ->
+        impl.f_repr out == Seq.create 16 0s);
+    f_ZERO = (fun (_: Prims.unit) -> Libcrux_ml_kem.Vector.Portable.Vector_type.zero ());
+    f_from_i16_array_pre
+    =
+    (fun (array: t_Slice i16) -> (Core.Slice.impl__len #i16 array <: usize) =. sz 16);
+    f_from_i16_array_post
+    =
+    (fun (array: t_Slice i16) (out: Libcrux_ml_kem.Vector.Portable.Vector_type.t_PortableVector) ->
+        impl.f_repr out == array);
+    f_from_i16_array
+    =
+    (fun (array: t_Slice i16) -> Libcrux_ml_kem.Vector.Portable.Vector_type.from_i16_array array);
     f_add_pre
     =
     (fun
